projects/lib/gmp_proof_manual.v
@@ -692,7 +692,7 @@ Proof.
   entailer!.
   rewrite H20.
   entailer!.
-  apply store_uint_array_rec_def2undef.
+  apply store_uint_array_rec_def2undef; try lia.
   assert (Zlength l' = n_pre) by lia.
   rewrite <- H7.
   tauto.
@@ -1261,7 +1261,7 @@ Proof.
   entailer!.
   rewrite H10.
   entailer!.
-  apply store_uint_array_rec_def2undef.
+  apply store_uint_array_rec_def2undef; try lia.
   rewrite <- H29.
   assert (val_a_prefix = val_a). {
     rewrite <-H18 in H7.
@@ -1709,6 +1709,77 @@ Proof.
 Qed.
 
 Lemma proof_of_mpz_sgn_which_implies_wit_1 : mpz_sgn_which_implies_wit_1.
+Proof.
+  pre_process.
+  unfold store_Z.
+  Intros ptr cap size.
+  rewrite orp_sepcon_left.
+  Split.
+  + Right.
+    Exists ptr cap size.
+    entailer!.
+  + Left.
+    Exists ptr cap size.
+    entailer!.
+Qed.
+
+Lemma proof_of_mpz_swap_return_wit_1_1 : mpz_swap_return_wit_1_1.
+Proof.
+  pre_process.
+  unfold store_Z.
+  Exists ptr2 cap2 size2.
+  Exists ptr1 cap1 size1.
+  Right; Right.
+  entailer!.
+Qed.
+
+Lemma proof_of_mpz_swap_return_wit_1_2 : mpz_swap_return_wit_1_2.
+Proof.
+  pre_process.
+  subst.
+  unfold store_Z.
+  Exists ptr2 cap2 size2.
+  Exists ptr1 cap1 size1.
+  Right; Left.
+  entailer!.
+Qed.
+
+Lemma proof_of_mpz_swap_return_wit_1_3 : mpz_swap_return_wit_1_3.
+Proof.
+  pre_process.
+  unfold store_Z.
+  Exists ptr2 cap2 size2.
+  Exists ptr1 cap1 size1.
+  Left; Right.
+  entailer!.
+Qed.
+
+Lemma proof_of_mpz_swap_return_wit_1_4 : mpz_swap_return_wit_1_4.
+Proof.
+  pre_process.
+  unfold store_Z.
+  Exists ptr2 cap2 size2.
+  Exists ptr1 cap1 size1.
+  Left; Left.
+  entailer!.
+Qed.
+
+Lemma proof_of_mpz_swap_which_implies_wit_1 : mpz_swap_which_implies_wit_1.
+Proof.
+  pre_process.
+  unfold store_Z.
+  Intros ptr cap size.
+  rewrite orp_sepcon_left.
+  Split.
+  + Right.
+    Exists ptr cap size.
+    entailer!.
+  + Left.
+    Exists ptr cap size.
+    entailer!.
+Qed.
+
+Lemma proof_of_mpz_swap_which_implies_wit_2 : mpz_swap_which_implies_wit_2.
 Proof.
   pre_process.
   unfold store_Z.
